Remove old implementation.

sheaves/fol/syntax.v
@@ -1,94 +1,410 @@
-Require Export fintype. Require Export header_extensible.
-
 Axiom symb : Set.
 Axiom symb_arity : symb -> nat.
 Axiom atom : Set.
 Axiom atom_arity : atom -> nat.
 
+Fixpoint fin (n : nat) : Type :=
+match n with
+| 0 => False
+| S m => option (fin m)
+end.
+
+Definition fin0 {n : nat} : fin (S n) := None.
+Definition finS {n : nat} (p : fin n) : fin (S n) := Some p.
+
+Notation var_zero := fin0.
+Notation shift := finS.
+
+Inductive seq (A : Type) : nat -> Type :=
+| seq0 : seq A 0
+| seqS : forall n, A -> seq A n -> seq A (S n).
+
+Notation null := seq0.
+Notation scons := seqS.
+
+Arguments seq0 {_}.
+Arguments seqS {_ _}.
+
+Definition seq_map {A B : Type} {n : nat} (f : A -> B) (v : seq A n) : seq B n :=
+(fix F n (v : seq A n) :=
+match v in seq _ n return seq B n with
+| seq0 => seq0
+| seqS x v => seqS (f x) (F _ v)
+end) n v.
+
+Lemma seq_map_map : forall {A B C} (n : nat) (f : A -> B) (g : B -> C) (v : seq A n),
+  seq_map g (seq_map f v) = seq_map (fun x => g (f x)) v.
+Proof.
+induction v; cbn; [reflexivity|].
+f_equal; apply IHv.
+Qed.
+
+Lemma seq_map_ext : forall {A B} (n : nat) (f g : A -> B) (v : seq A n),
+  (forall x : A, f x = g x) -> seq_map f v = seq_map g v.
+Proof.
+induction v; intros H; cbn; [reflexivity|].
+f_equal; [apply H|]; apply IHv, H.
+Qed.
+
+Fixpoint seq_init {A} {n : nat} (f : fin n -> A) : seq A n :=
+match n return (fin n -> A) -> seq A n with
+| 0 => fun _ => seq0
+| S n => fun f => seqS (f var_zero) (@seq_init A n (fun p => f (finS p)))
+end f.
+
+Lemma map_init : forall A B n (f : fin n -> A) (g : A -> B),
+  seq_map g (seq_init f) = seq_init (fun p => g (f p)).
+Proof.
+induction n; intros f g; simpl; [reflexivity|].
+f_equal; apply IHn.
+Qed.
+
+Definition hd {A} {n : nat} (v : seq A (S n)) : A :=
+match v in seq _ n return
+  match n with 0 => unit | S n => A end
+with
+| seq0 => tt
+| seqS x v => x 
+end.
+
+Definition tl {A} {n : nat} (v : seq A (S n)) : seq A n :=
+match v in seq _ n return
+  match n with 0 => unit | S n => seq A n end
+with
+| seq0 => tt
+| seqS x v => v 
+end.
+
+Fixpoint tl_n {A n} (p : nat) : seq A (p + n) -> seq A n :=
+match p return seq A (p + n) -> seq A n with
+| 0 => fun v => v
+| S p => fun v => tl_n p (tl v)
+end.
+
+Fixpoint hd_n {A n} (p : nat) : seq A (p + n) -> seq A p :=
+match p return seq A (p + n) -> seq A p with
+| 0 => fun v => seq0
+| S p => fun v =>
+  match v in seq _ n return
+    match n with 0 => unit | S n => (seq A n -> _) -> seq A (S p) end
+  with
+  | seq0 => tt
+  | seqS x v => fun k => seqS x (k v)
+  end (hd_n p)
+end.
+
+Fixpoint seq_app {A m n} (v : seq A m) (w : seq A n) : seq A (m + n) :=
+match v in seq _ m return seq A n -> seq A (m + n) with
+| seq0 => fun w => w
+| seqS x v => fun w => seqS x (seq_app v w)
+end w.
+
+Lemma seq0_eta : forall A (v : seq A 0), v = seq0.
+Proof.
+intros A v.
+refine (
+match v in seq _ n return
+  match n return seq A n -> Prop with
+  | 0 => fun v => v = seq0
+  | S n => fun _ => True
+  end v
+with
+| seq0 => eq_refl
+| seqS _ _ => I
+end
+).
+Qed.
+
+Lemma hd_tl : forall A (n : nat) (v : seq A (S n)), v = seqS (hd v) (tl v).
+Proof.
+intros A n v. 
+refine (
+match v in seq _ n return
+  match n return seq A n -> Prop with
+  | 0 => fun _ => True
+  | S n => fun (v : seq A (S n)) => v = seqS (hd v) (tl v)
+  end v
+ with
+| seq0 => I
+| seqS x v => eq_refl
+end
+).
+Qed.
+
+Lemma hd_tl_n : forall A (p n : nat) (v : seq A (p + n)),
+  seq_app (hd_n p v) (tl_n p v) = v.
+Proof.
+induction p; intros n v; cbn in *; [reflexivity|].
+rewrite (hd_tl _ _ v); cbn; rewrite IHp; reflexivity.
+Qed.
+
+Fixpoint nth {A n} (v : seq A n) : fin n -> A :=
+match v in seq _ n return fin n -> A with
+| seq0 =>
+  fun p => match p with end
+| seqS x v =>
+  fun p => match p with
+  | None => x
+  | Some p => nth v p
+  end
+end.
+
+Lemma nth_init : forall A (n : nat) (f : fin n -> A) p, nth (seq_init f) p = f p.
+Proof.
+induction n; cbn.
++ intros f [].
++ intros f [p|]; [|reflexivity].
+  apply IHn.
+Qed.
+
+Lemma nth_map : forall A B (n : nat) (f : A -> B) (v : seq A n) (p : fin n),
+  nth (seq_map f v) p = f (nth v p).
+Proof.
+induction v; cbn.
++ intros [].
++ intros [p|]; [|reflexivity].
+  apply IHv.
+Qed.
+
+Lemma nth_ext : forall A n (v w : seq A n),
+  (forall p : fin n, nth v p = nth w p) -> v = w.
+Proof.
+induction n; intros v w e.
++ rewrite (seq0_eta _ v), (seq0_eta _ w); reflexivity.
++ rewrite (hd_tl _ _ v), (hd_tl _ _ w); f_equal.
+  - specialize (e None); cbn in e.
+    rewrite (hd_tl _ _ v), (hd_tl _ _ w) in e; exact e.
+  - apply IHn; intros p.
+    specialize (e (Some p)); cbn in e.
+    rewrite (hd_tl _ _ v), (hd_tl _ _ w) in e; exact e.
+Qed.
+
+Fixpoint zero_p (m : nat) {n : nat} : fin m -> fin (m + n) :=
+match m return fin m -> fin (m + n) with
+| 0 => fun p => match p with end
+| S m => fun p => match p with None => var_zero | Some p => Some (zero_p m p) end
+end.
+
+Fixpoint shift_p (m : nat) {n : nat} (p : fin n) : fin (m + n) :=
+match m return fin (m + n) with
+| 0 => p
+| S m => finS (shift_p m p)
+end.
+
+Lemma fin_add_rect : forall m n (P : fin (m + n) -> Type),
+  (forall p : fin m, P (zero_p _ p)) ->
+  (forall p : fin n, P (shift_p _ p)) ->
+  forall p : fin (m + n), P p.
+Proof.
+induction m as [|m IHm]; intros n P Hm Hn p; cbn in *.
++ apply Hn.
++ destruct p as [p|].
+  - apply (IHm n (fun p => P (Some p)) (fun p => Hm (Some p)) Hn).
+  - apply (Hm None).
+Defined.
+
+Lemma nth_zero_p : forall A m n (v : seq A m) (w : seq A n) (p : fin m),
+  nth (seq_app v w) (zero_p _ p) = nth v p.
+Proof.
+induction m; intros n v w p; cbn in *.
++ destruct p.
++ destruct p as [p|]; cbn.
+  - rewrite (hd_tl _ _ v); cbn.
+    apply IHm.
+  - rewrite (hd_tl _ _ v); reflexivity.
+Qed.
+
+Lemma nth_shift_p : forall A m n (v : seq A m) (w : seq A n) (p : fin n),
+  nth (seq_app v w) (shift_p _ p) = nth w p.
+Proof.
+induction m; intros n v w p; cbn in *.
++ replace v with (@seq0 A); [reflexivity|].
+  symmetry; apply seq0_eta.
++ rewrite (hd_tl _ _ v); cbn.
+  apply IHm.
+Qed.
+
+Notation scons_p := seq_app.
+
+
 Section term.
+
+
+Unset Elimination Schemes.
 Inductive term (nterm : nat) : Type :=
-  | var_term : (fin) (nterm) -> term (nterm)
-  | App
-  : forall (s : symb), cod (fin (symb_arity s)) (term  (nterm)) -> term (nterm).
+| var_term : fin nterm -> term nterm
+| App : forall (s : symb) (l : seq (term (nterm)) (symb_arity s)), term (nterm).
+Set Elimination Schemes.
 
-Lemma congr_App { s : symb } { mterm : nat } { s0 : cod (fin (symb_arity s)) (term  (mterm)) } { t0 : cod (fin (symb_arity s)) (term  (mterm)) } (H1 : s0 = t0) : App (mterm) s s0 = App (mterm) s t0 .
-Proof. congruence. Qed.
+Lemma term_rect : forall (n : nat) (P : term n -> Type)
+  (pvar : forall f : fin n, P (var_term n f))
+  (papp : forall (s : symb) (l : seq (term n) (symb_arity s)), (forall p, P (nth l p)) -> P (App n s l)),
+  forall t : term n, P t.
+Proof.
+intros n P pvar papp.
+simple refine (
+fix F t :=
+match t return P t with
+| var_term _ p => pvar _
+| App _ s l => papp _ _ (fun p => _)
+end 
+).
+refine (
+(fix G (m : nat) (l : seq (term n) m) {struct l} : forall (p : fin m), P (nth l p) :=
+match l in seq _ m return forall p : fin m, P (nth l p) with
+| seq0 => fun p => match p with end
+| seqS x l =>
+  fun p => match p return (forall p, P (nth l p)) -> P (nth (seqS x l) p) with
+  | None => fun _ => F x
+  | Some p => fun G => G p
+  end (G _ l)
+end
+) _ l p).
+Defined.
 
-Fixpoint subst_term { mterm : nat } { nterm : nat } (sigmaterm : (fin) (mterm) -> term (nterm)) (s : term (mterm)) : term (nterm) :=
-    match s with
-    | var_term (_) s => sigmaterm s
-    | App (_) s s0 => App (nterm) s ((cod_map (subst_term sigmaterm)) s0)
-    end.
+Definition term_ind (n : nat) (P : term n -> Type)
+  (pvar : forall f : fin n, P (var_term n f))
+  (papp : forall (s : symb) (l : seq (term n) (symb_arity s)), (forall p, P (nth l p)) -> P (App n s l))
+  (t : term n) : P t :=
+  term_rect n P pvar papp t.
 
-Definition up_term_term { m : nat } { nterm : nat } (sigma : (fin) (m) -> term (nterm)) : (fin) ((S) (m)) -> term ((S) nterm) :=
-  (scons) ((var_term ((S) nterm)) (var_zero)) ((funcomp) (subst_term ((funcomp) (var_term (_)) (shift))) sigma).
+Fixpoint subst_term { mterm : nat } { nterm : nat } (sigmaterm : seq (term (nterm)) mterm)  (s : term (mterm)) {struct s} : term (nterm) :=
+match s with
+| var_term (_) s => nth sigmaterm s
+| App (_) s s0 => App (nterm) s (seq_map (subst_term sigmaterm) s0)
+end.
 
-Definition upList_term_term (p : nat) { m : nat } { nterm : nat } (sigma : (fin) (m) -> term (nterm)) : (fin) (p+ (m)) -> term (p+ nterm) :=
-  scons_p  p ((funcomp) (var_term (p+ nterm)) (zero_p p)) ((funcomp) (subst_term ((funcomp) (var_term (_)) (shift_p p))) sigma).
+Definition funcomp {A B C} (g : B -> C) (f : A -> B) (x : A) : C := g (f x).
 
-Definition upId_term_term { mterm : nat } (sigma : (fin) (mterm) -> term (mterm)) (Eq : forall x, sigma x = (var_term (mterm)) x) : forall x, (up_term_term sigma) x = (var_term ((S) mterm)) x :=
-  fun n => match n with
-  | Some fin_n => (ap) (subst_term ((funcomp) (var_term (_)) (shift))) (Eq fin_n)
-  | None => eq_refl
-  end.
+Definition up_term_term { m : nat } { nterm : nat } (sigma : seq (term nterm) m) : seq (term (S nterm)) (S m).
+Proof.
+simple refine (seqS ((var_term (S nterm)) (var_zero)) _).
+simple refine (seq_map (subst_term _) sigma).
+refine (seq_init (funcomp (var_term _) shift)).
+Defined.
 
-Definition upIdList_term_term { p : nat } { mterm : nat } (sigma : (fin) (mterm) -> term (mterm)) (Eq : forall x, sigma x = (var_term (mterm)) x) : forall x, (upList_term_term p sigma) x = (var_term (p+ mterm)) x :=
-  fun n => scons_p_eta (var_term (p+ mterm)) (fun n => (ap) (subst_term ((funcomp) (var_term (_)) (shift_p p))) (Eq n)) (fun n => eq_refl).
+Definition upList_term_term (p : nat) { m : nat } { nterm : nat } (sigma : seq (term (nterm)) m) : seq (term (p+ nterm)) (p + m).
+Proof.
+simple refine (scons_p _ _).
++ refine (seq_init (((funcomp) (var_term (p+ nterm)) (zero_p p)))).
++ refine (seq_map _ sigma).
+  refine ((subst_term (seq_init ((funcomp) (var_term (_)) (shift_p p))))).
+Defined.
 
-Fixpoint idSubst_term { mterm : nat } (sigmaterm : (fin) (mterm) -> term (mterm)) (Eqterm : forall x, sigmaterm x = (var_term (mterm)) x) (s : term (mterm)) : subst_term sigmaterm s = s :=
-    match s with
-    | var_term (_) s => Eqterm s
-    | App (_) s s0 => congr_App ((cod_id (idSubst_term sigmaterm Eqterm)) s0)
-    end.
+Definition upId_term_term { mterm : nat }
+  (sigma : seq (term (mterm)) mterm)
+  (Eq : forall x, nth sigma x = (var_term (mterm)) x) :
+  forall x, nth (up_term_term sigma) x = (var_term ((S) mterm)) x.
+Proof.
+intros [n|]; [|reflexivity].
+unfold up_term_term; cbn.
+rewrite nth_map; cbn.
+rewrite Eq; cbn; rewrite nth_init; cbn; reflexivity.
+Qed.
 
-Definition upExt_term_term { m : nat } { nterm : nat } (sigma : (fin) (m) -> term (nterm)) (tau : (fin) (m) -> term (nterm)) (Eq : forall x, sigma x = tau x) : forall x, (up_term_term sigma) x = (up_term_term tau) x :=
-  fun n => match n with
-  | Some fin_n => (ap) (subst_term ((funcomp) (var_term (_)) (shift))) (Eq fin_n)
-  | None => eq_refl
-  end.
+Definition upIdList_term_term { p : nat } { mterm : nat }
+  (sigma : seq (term mterm) mterm)
+  (Eq : forall x, nth sigma x = (var_term (mterm)) x) :
+  forall x, nth (upList_term_term p sigma) x = (var_term (p + mterm)) x.
+Proof.
+apply fin_add_rect; intros n; unfold upList_term_term; cbn.
++ rewrite nth_zero_p; cbn.
+  rewrite nth_init; reflexivity.
++ rewrite nth_shift_p; cbn.
+  rewrite nth_map, Eq; cbn.
+  rewrite nth_init; reflexivity.
+Qed.
 
-Definition upExt_list_term_term { p : nat } { m : nat } { nterm : nat } (sigma : (fin) (m) -> term (nterm)) (tau : (fin) (m) -> term (nterm)) (Eq : forall x, sigma x = tau x) : forall x, (upList_term_term p sigma) x = (upList_term_term p tau) x :=
-  fun n => scons_p_congr (fun n => eq_refl) (fun n => (ap) (subst_term ((funcomp) (var_term (_)) (shift_p p))) (Eq n)).
+Fixpoint idSubst_term { mterm : nat }
+  (sigmaterm : seq (term mterm) mterm)
+  (Eqterm : forall x, nth sigmaterm x = (var_term (mterm)) x)
+  (s : term (mterm)) : subst_term sigmaterm s = s.
+Proof.
+induction s.
++ apply Eqterm.
++ cbn; f_equal; apply nth_ext.
+  intros p.
+  rewrite nth_map; apply H.
+Qed.
 
-Fixpoint ext_term { mterm : nat } { nterm : nat } (sigmaterm : (fin) (mterm) -> term (nterm)) (tauterm : (fin) (mterm) -> term (nterm)) (Eqterm : forall x, sigmaterm x = tauterm x) (s : term (mterm)) : subst_term sigmaterm s = subst_term tauterm s :=
-    match s with
-    | var_term (_) s => Eqterm s
-    | App (_) s s0 => congr_App ((cod_ext (ext_term sigmaterm tauterm Eqterm)) s0)
-    end.
+Lemma compSubstSubst_term { kterm : nat } { lterm : nat } { mterm : nat }
+  (sigmaterm : seq (term (kterm)) mterm)
+  (tauterm : seq  (term (lterm)) kterm)
+  (thetaterm : seq (term (lterm)) mterm)
+  (Eqterm : seq_map (subst_term tauterm) sigmaterm = thetaterm)
+  (s : term (mterm)) :
+    subst_term tauterm (subst_term sigmaterm s) = subst_term thetaterm s.
+Proof.
+induction s; cbn.
++ rewrite <- Eqterm, nth_map; reflexivity.
++ f_equal; rewrite seq_map_map; apply nth_ext; intros p.
+  rewrite nth_map, H, nth_map; reflexivity.
+Qed.
 
-Fixpoint compSubstSubst_term { kterm : nat } { lterm : nat } { mterm : nat } (sigmaterm : (fin) (mterm) -> term (kterm)) (tauterm : (fin) (kterm) -> term (lterm)) (thetaterm : (fin) (mterm) -> term (lterm)) (Eqterm : forall x, ((funcomp) (subst_term tauterm) sigmaterm) x = thetaterm x) (s : term (mterm)) : subst_term tauterm (subst_term sigmaterm s) = subst_term thetaterm s :=
-    match s with
-    | var_term (_) s => Eqterm s
-    | App (_) s s0 => congr_App ((cod_comp (compSubstSubst_term sigmaterm tauterm thetaterm Eqterm)) s0)
-    end.
+Definition up_subst_subst_term_term { k : nat } { lterm : nat } { mterm : nat }
+  (sigma : seq (term (lterm)) k)
+  (tauterm : seq  (term (mterm)) lterm)
+  (theta : seq (term (mterm)) k)
+  (Eq : (seq_map (subst_term tauterm) sigma) = theta) :
+  (seq_map (subst_term (up_term_term tauterm)) (up_term_term sigma)) = (up_term_term theta).
+Proof.
+apply nth_ext; intros [p|].
++ rewrite nth_map; simpl.
+  rewrite !nth_map.
+  etransitivity; [apply compSubstSubst_term; reflexivity|].
+  rewrite <- Eq, !nth_map.
+  etransitivity; [|symmetry; apply compSubstSubst_term; reflexivity].
+  f_equal; apply nth_ext; clear p; intro p.
+  rewrite !nth_map, nth_init.
+  unfold funcomp; simpl; rewrite !nth_map; reflexivity.
++ reflexivity.
+Qed.
 
-Definition up_subst_subst_term_term { k : nat } { lterm : nat } { mterm : nat } (sigma : (fin) (k) -> term (lterm)) (tauterm : (fin) (lterm) -> term (mterm)) (theta : (fin) (k) -> term (mterm)) (Eq : forall x, ((funcomp) (subst_term tauterm) sigma) x = theta x) : forall x, ((funcomp) (subst_term (up_term_term tauterm)) (up_term_term sigma)) x = (up_term_term theta) x :=
-  fun n => match n with
-  | Some fin_n => (eq_trans) (compSubstSubst_term ((funcomp) (var_term (_)) (shift)) (up_term_term tauterm) ((funcomp) (up_term_term tauterm) (shift)) (fun x => eq_refl) (sigma fin_n)) ((eq_trans) ((eq_sym) (compSubstSubst_term tauterm ((funcomp) (var_term (_)) (shift)) ((funcomp) (subst_term ((funcomp) (var_term (_)) (shift))) tauterm) (fun x => eq_refl) (sigma fin_n))) ((ap) (subst_term ((funcomp) (var_term (_)) (shift))) (Eq fin_n)))
-  | None => eq_refl
-  end.
+Definition up_subst_subst_list_term_term { p : nat } { k : nat } { lterm : nat } { mterm : nat }
+  (sigma : seq (term (lterm)) k)
+  (tauterm : seq (term (mterm)) lterm)
+  (theta : seq (term (mterm)) k)
+  (Eq : (seq_map (subst_term tauterm) sigma) = theta) :
+  (seq_map (subst_term (upList_term_term p tauterm)) (upList_term_term p sigma)) = (upList_term_term p theta).
+Proof.
+apply nth_ext; apply fin_add_rect; intros q.
++ rewrite nth_map.
+  unfold upList_term_term.
+  rewrite !nth_zero_p, !nth_init; simpl; rewrite nth_zero_p, nth_init; reflexivity.
++ rewrite nth_map.
+  unfold upList_term_term.
+  rewrite !nth_shift_p, !nth_map; simpl.
+  rewrite <- Eq, !nth_map.
+  etransitivity; [apply compSubstSubst_term; reflexivity|].
+  symmetry; apply compSubstSubst_term.
+  rewrite map_init; apply nth_ext; clear q; intro q.
+  rewrite !nth_map, !nth_init; cbn.
+  rewrite nth_shift_p, nth_map; reflexivity.
+Qed.
 
-Definition up_subst_subst_list_term_term { p : nat } { k : nat } { lterm : nat } { mterm : nat } (sigma : (fin) (k) -> term (lterm)) (tauterm : (fin) (lterm) -> term (mterm)) (theta : (fin) (k) -> term (mterm)) (Eq : forall x, ((funcomp) (subst_term tauterm) sigma) x = theta x) : forall x, ((funcomp) (subst_term (upList_term_term p tauterm)) (upList_term_term p sigma)) x = (upList_term_term p theta) x :=
-  fun n => (eq_trans) (scons_p_comp' ((funcomp) (var_term (p+ lterm)) (zero_p p)) (_) (_) n) (scons_p_congr (fun x => scons_p_head' (_) (fun z => subst_term ((funcomp) (var_term (_)) (shift_p p)) (_)) x) (fun n => (eq_trans) (compSubstSubst_term ((funcomp) (var_term (_)) (shift_p p)) (upList_term_term p tauterm) ((funcomp) (upList_term_term p tauterm) (shift_p p)) (fun x => eq_refl) (sigma n)) ((eq_trans) ((eq_sym) (compSubstSubst_term tauterm ((funcomp) (var_term (_)) (shift_p p)) (_) (fun x => (eq_sym) (scons_p_tail' (_) (_) x)) (sigma n))) ((ap) (subst_term ((funcomp) (var_term (_)) (shift_p p))) (Eq n))))).
+Lemma varL_term { mterm : nat } { nterm : nat }
+  (sigmaterm : seq (term (nterm)) mterm) :
+    seq_map (subst_term sigmaterm) (seq_init (var_term (mterm))) = sigmaterm.
+Proof.
+rewrite map_init; apply nth_ext; intros p; rewrite nth_init; reflexivity.
+Qed.
 
-Lemma instId_term { mterm : nat } : subst_term (var_term (mterm)) = id .
-Proof. exact ((FunctionalExtensionality.functional_extensionality _ _ ) (fun x => idSubst_term (var_term (mterm)) (fun n => eq_refl) ((id) x))). Qed.
-
-Lemma varL_term { mterm : nat } { nterm : nat } (sigmaterm : (fin) (mterm) -> term (nterm)) : (funcomp) (subst_term sigmaterm) (var_term (mterm)) = sigmaterm .
-Proof. exact ((FunctionalExtensionality.functional_extensionality _ _ ) (fun x => eq_refl)). Qed.
-
-Lemma compComp_term { kterm : nat } { lterm : nat } { mterm : nat } (sigmaterm : (fin) (mterm) -> term (kterm)) (tauterm : (fin) (kterm) -> term (lterm)) (s : term (mterm)) : subst_term tauterm (subst_term sigmaterm s) = subst_term ((funcomp) (subst_term tauterm) sigmaterm) s .
-Proof. exact (compSubstSubst_term sigmaterm tauterm (_) (fun n => eq_refl) s). Qed.
-
-Lemma compComp'_term { kterm : nat } { lterm : nat } { mterm : nat } (sigmaterm : (fin) (mterm) -> term (kterm)) (tauterm : (fin) (kterm) -> term (lterm)) : (funcomp) (subst_term tauterm) (subst_term sigmaterm) = subst_term ((funcomp) (subst_term tauterm) sigmaterm) .
-Proof. exact ((FunctionalExtensionality.functional_extensionality _ _ ) (fun n => compComp_term sigmaterm tauterm n)). Qed.
+Lemma compComp_term { kterm : nat } { lterm : nat } { mterm : nat }
+  (sigmaterm : seq (term (kterm)) mterm)
+  (tauterm : seq (term (lterm)) kterm)
+  (s : term (mterm)) :
+    subst_term tauterm (subst_term sigmaterm s) = subst_term (seq_map (subst_term tauterm) sigmaterm) s.
+Proof.
+apply compSubstSubst_term; reflexivity.
+Qed.
 
 End term.
 
 Section form.
+
 Inductive form (nterm : nat) : Type :=
   | Atm
-  : forall (a : atom), cod (fin (atom_arity a)) (term  (nterm)) -> form (nterm)
+  : forall (a : atom), seq (term  (nterm)) (atom_arity a) -> form (nterm)
   | Arr : form  (nterm) -> form  (nterm) -> form (nterm)
   | Top : form (nterm)
   | Bot : form (nterm)
@@ -97,33 +413,9 @@ Inductive form (nterm : nat) : Type :=
   | All : form  ((S) nterm) -> form (nterm)
   | Exs : form  ((S) nterm) -> form (nterm).
 
-Lemma congr_Atm { a : atom } { mterm : nat } { s0 : cod (fin (atom_arity a)) (term  (mterm)) } { t0 : cod (fin (atom_arity a)) (term  (mterm)) } (H1 : s0 = t0) : Atm (mterm) a s0 = Atm (mterm) a t0 .
-Proof. congruence. Qed.
-
-Lemma congr_Arr { mterm : nat } { s0 : form  (mterm) } { s1 : form  (mterm) } { t0 : form  (mterm) } { t1 : form  (mterm) } (H1 : s0 = t0) (H2 : s1 = t1) : Arr (mterm) s0 s1 = Arr (mterm) t0 t1 .
-Proof. congruence. Qed.
-
-Lemma congr_Top { mterm : nat } : Top (mterm) = Top (mterm) .
-Proof. congruence. Qed.
-
-Lemma congr_Bot { mterm : nat } : Bot (mterm) = Bot (mterm) .
-Proof. congruence. Qed.
-
-Lemma congr_Cnj { mterm : nat } { s0 : form  (mterm) } { s1 : form  (mterm) } { t0 : form  (mterm) } { t1 : form  (mterm) } (H1 : s0 = t0) (H2 : s1 = t1) : Cnj (mterm) s0 s1 = Cnj (mterm) t0 t1 .
-Proof. congruence. Qed.
-
-Lemma congr_Dsj { mterm : nat } { s0 : form  (mterm) } { s1 : form  (mterm) } { t0 : form  (mterm) } { t1 : form  (mterm) } (H1 : s0 = t0) (H2 : s1 = t1) : Dsj (mterm) s0 s1 = Dsj (mterm) t0 t1 .
-Proof. congruence. Qed.
-
-Lemma congr_All { mterm : nat } { s0 : form  ((S) mterm) } { t0 : form  ((S) mterm) } (H1 : s0 = t0) : All (mterm) s0 = All (mterm) t0 .
-Proof. congruence. Qed.
-
-Lemma congr_Exs { mterm : nat } { s0 : form  ((S) mterm) } { t0 : form  ((S) mterm) } (H1 : s0 = t0) : Exs (mterm) s0 = Exs (mterm) t0 .
-Proof. congruence. Qed.
-
-Fixpoint subst_form { mterm : nat } { nterm : nat } (sigmaterm : (fin) (mterm) -> term (nterm)) (s : form (mterm)) : form (nterm) :=
+Fixpoint subst_form { mterm : nat } { nterm : nat } (sigmaterm : seq (term (nterm)) mterm) (s : form (mterm)) : form (nterm) :=
     match s with
-    | Atm (_) a s0 => Atm (nterm) a ((cod_map (subst_term sigmaterm)) s0)
+    | Atm (_) a s0 => Atm (nterm) a ((seq_map (subst_term sigmaterm)) s0)
     | Arr (_) s0 s1 => Arr (nterm) ((subst_form sigmaterm) s0) ((subst_form sigmaterm) s1)
     | Top (_)  => Top (nterm)
     | Bot (_)  => Bot (nterm)
@@ -133,50 +425,36 @@ Fixpoint subst_form { mterm : nat } { nterm : nat } (sigmaterm : (fin) (mterm) -
     | Exs (_) s0 => Exs (nterm) ((subst_form (up_term_term sigmaterm)) s0)
     end.
 
-Fixpoint idSubst_form { mterm : nat } (sigmaterm : (fin) (mterm) -> term (mterm)) (Eqterm : forall x, sigmaterm x = (var_term (mterm)) x) (s : form (mterm)) : subst_form sigmaterm s = s :=
-    match s with
-    | Atm (_) a s0 => congr_Atm ((cod_id (idSubst_term sigmaterm Eqterm)) s0)
-    | Arr (_) s0 s1 => congr_Arr ((idSubst_form sigmaterm Eqterm) s0) ((idSubst_form sigmaterm Eqterm) s1)
-    | Top (_)  => congr_Top 
-    | Bot (_)  => congr_Bot 
-    | Cnj (_) s0 s1 => congr_Cnj ((idSubst_form sigmaterm Eqterm) s0) ((idSubst_form sigmaterm Eqterm) s1)
-    | Dsj (_) s0 s1 => congr_Dsj ((idSubst_form sigmaterm Eqterm) s0) ((idSubst_form sigmaterm Eqterm) s1)
-    | All (_) s0 => congr_All ((idSubst_form (up_term_term sigmaterm) (upId_term_term (_) Eqterm)) s0)
-    | Exs (_) s0 => congr_Exs ((idSubst_form (up_term_term sigmaterm) (upId_term_term (_) Eqterm)) s0)
-    end.
+Lemma idSubst_form { mterm : nat }
+  (sigmaterm : seq (term (mterm)) mterm)
+  (Eqterm : forall x, nth sigmaterm x = (var_term (mterm)) x) (s : form (mterm)) :
+    subst_form sigmaterm s = s.
+Proof.
+induction s; simpl; f_equal; try match goal with [ H : _ |- _] => solve [apply H; assumption] end.
++ apply nth_ext; intros p; rewrite nth_map.
+  apply idSubst_term; assumption.
++ apply IHs; apply upId_term_term, Eqterm.
++ apply IHs; apply upId_term_term, Eqterm.
+Qed.
 
-Fixpoint ext_form { mterm : nat } { nterm : nat } (sigmaterm : (fin) (mterm) -> term (nterm)) (tauterm : (fin) (mterm) -> term (nterm)) (Eqterm : forall x, sigmaterm x = tauterm x) (s : form (mterm)) : subst_form sigmaterm s = subst_form tauterm s :=
-    match s with
-    | Atm (_) a s0 => congr_Atm ((cod_ext (ext_term sigmaterm tauterm Eqterm)) s0)
-    | Arr (_) s0 s1 => congr_Arr ((ext_form sigmaterm tauterm Eqterm) s0) ((ext_form sigmaterm tauterm Eqterm) s1)
-    | Top (_)  => congr_Top 
-    | Bot (_)  => congr_Bot 
-    | Cnj (_) s0 s1 => congr_Cnj ((ext_form sigmaterm tauterm Eqterm) s0) ((ext_form sigmaterm tauterm Eqterm) s1)
-    | Dsj (_) s0 s1 => congr_Dsj ((ext_form sigmaterm tauterm Eqterm) s0) ((ext_form sigmaterm tauterm Eqterm) s1)
-    | All (_) s0 => congr_All ((ext_form (up_term_term sigmaterm) (up_term_term tauterm) (upExt_term_term (_) (_) Eqterm)) s0)
-    | Exs (_) s0 => congr_Exs ((ext_form (up_term_term sigmaterm) (up_term_term tauterm) (upExt_term_term (_) (_) Eqterm)) s0)
-    end.
-
-Fixpoint compSubstSubst_form { kterm : nat } { lterm : nat } { mterm : nat } (sigmaterm : (fin) (mterm) -> term (kterm)) (tauterm : (fin) (kterm) -> term (lterm)) (thetaterm : (fin) (mterm) -> term (lterm)) (Eqterm : forall x, ((funcomp) (subst_term tauterm) sigmaterm) x = thetaterm x) (s : form (mterm)) : subst_form tauterm (subst_form sigmaterm s) = subst_form thetaterm s :=
-    match s with
-    | Atm (_) a s0 => congr_Atm ((cod_comp (compSubstSubst_term sigmaterm tauterm thetaterm Eqterm)) s0)
-    | Arr (_) s0 s1 => congr_Arr ((compSubstSubst_form sigmaterm tauterm thetaterm Eqterm) s0) ((compSubstSubst_form sigmaterm tauterm thetaterm Eqterm) s1)
-    | Top (_)  => congr_Top 
-    | Bot (_)  => congr_Bot 
-    | Cnj (_) s0 s1 => congr_Cnj ((compSubstSubst_form sigmaterm tauterm thetaterm Eqterm) s0) ((compSubstSubst_form sigmaterm tauterm thetaterm Eqterm) s1)
-    | Dsj (_) s0 s1 => congr_Dsj ((compSubstSubst_form sigmaterm tauterm thetaterm Eqterm) s0) ((compSubstSubst_form sigmaterm tauterm thetaterm Eqterm) s1)
-    | All (_) s0 => congr_All ((compSubstSubst_form (up_term_term sigmaterm) (up_term_term tauterm) (up_term_term thetaterm) (up_subst_subst_term_term (_) (_) (_) Eqterm)) s0)
-    | Exs (_) s0 => congr_Exs ((compSubstSubst_form (up_term_term sigmaterm) (up_term_term tauterm) (up_term_term thetaterm) (up_subst_subst_term_term (_) (_) (_) Eqterm)) s0)
-    end.
-
-Lemma instId_form { mterm : nat } : subst_form (var_term (mterm)) = id .
-Proof. exact ((FunctionalExtensionality.functional_extensionality _ _ ) (fun x => idSubst_form (var_term (mterm)) (fun n => eq_refl) ((id) x))). Qed.
-
-Lemma compComp_form { kterm : nat } { lterm : nat } { mterm : nat } (sigmaterm : (fin) (mterm) -> term (kterm)) (tauterm : (fin) (kterm) -> term (lterm)) (s : form (mterm)) : subst_form tauterm (subst_form sigmaterm s) = subst_form ((funcomp) (subst_term tauterm) sigmaterm) s .
-Proof. exact (compSubstSubst_form sigmaterm tauterm (_) (fun n => eq_refl) s). Qed.
-
-Lemma compComp'_form { kterm : nat } { lterm : nat } { mterm : nat } (sigmaterm : (fin) (mterm) -> term (kterm)) (tauterm : (fin) (kterm) -> term (lterm)) : (funcomp) (subst_form tauterm) (subst_form sigmaterm) = subst_form ((funcomp) (subst_term tauterm) sigmaterm) .
-Proof. exact ((FunctionalExtensionality.functional_extensionality _ _ ) (fun n => compComp_form sigmaterm tauterm n)). Qed.
+Lemma compSubstSubst_form { kterm : nat } { lterm : nat } { mterm : nat }
+  (sigmaterm : seq (term (kterm)) mterm)
+  (tauterm : seq (term (lterm)) kterm)
+  (thetaterm : seq (term (lterm)) mterm)
+  (Eqterm : (seq_map (subst_term tauterm) sigmaterm) = thetaterm)
+  (s : form (mterm)) :
+    subst_form tauterm (subst_form sigmaterm s) = subst_form thetaterm s.
+Proof.
+revert kterm lterm sigmaterm tauterm thetaterm Eqterm.
+induction s; intros kterm lterm sigmaterm tauterm thetaterm Eqterm;
+simpl; f_equal; try match goal with [ H : _ |- _] => solve [apply H; assumption] end.
++ rewrite seq_map_map; apply seq_map_ext; intros p.
+  apply compSubstSubst_term; assumption.
++ apply IHs.
+  apply up_subst_subst_term_term, Eqterm.
++ apply IHs.
+  apply up_subst_subst_term_term, Eqterm.
+Qed.
 
 End form.
 
@@ -200,48 +478,4 @@ Arguments All {nterm}.
 
 Arguments Exs {nterm}.
 
-Global Instance Subst_term { mterm : nat } { nterm : nat } : Subst1 ((fin) (mterm) -> term (nterm)) (term (mterm)) (term (nterm)) := @subst_term (mterm) (nterm) .
-
-Global Instance Subst_form { mterm : nat } { nterm : nat } : Subst1 ((fin) (mterm) -> term (nterm)) (form (mterm)) (form (nterm)) := @subst_form (mterm) (nterm) .
-
-Global Instance VarInstance_term { mterm : nat } : Var ((fin) (mterm)) (term (mterm)) := @var_term (mterm) .
-
-Notation "x '__term'" := (var_term x) (at level 5, format "x __term") : subst_scope.
-
-Notation "x '__term'" := (@ids (_) (_) VarInstance_term x) (at level 5, only printing, format "x __term") : subst_scope.
-
-Notation "'var'" := (var_term) (only printing, at level 1) : subst_scope.
-
-Class Up_term X Y := up_term : X -> Y.
-
-Notation "↑__term" := (up_term) (only printing) : subst_scope.
-
-Notation "↑__term" := (up_term_term) (only printing) : subst_scope.
-
-Global Instance Up_term_term { m : nat } { nterm : nat } : Up_term (_) (_) := @up_term_term (m) (nterm) .
-
-Notation "s [ sigmaterm ]" := (subst_term sigmaterm s) (at level 7, left associativity, only printing) : subst_scope.
-
-Notation "[ sigmaterm ]" := (subst_term sigmaterm) (at level 1, left associativity, only printing) : fscope.
-
-Notation "s [ sigmaterm ]" := (subst_form sigmaterm s) (at level 7, left associativity, only printing) : subst_scope.
-
-Notation "[ sigmaterm ]" := (subst_form sigmaterm) (at level 1, left associativity, only printing) : fscope.
-
-Ltac auto_unfold := repeat unfold subst1,  subst2,  Subst1,  Subst2,  ids,  ren1,  ren2,  Ren1,  Ren2,  Subst_term,  Subst_form,  VarInstance_term.
-
-Tactic Notation "auto_unfold" "in" "*" := repeat unfold subst1,  subst2,  Subst1,  Subst2,  ids,  ren1,  ren2,  Ren1,  Ren2,  Subst_term,  Subst_form,  VarInstance_term in *.
-
-Ltac asimpl' := repeat first [progress rewrite ?instId_term| progress rewrite ?compComp_term| progress rewrite ?compComp'_term| progress rewrite ?instId_form| progress rewrite ?compComp_form| progress rewrite ?compComp'_form| progress rewrite ?varL_term| progress (unfold up_ren, up_term_term, upList_term_term)| progress (cbn [subst_term subst_form])| fsimpl].
-
-Ltac asimpl := repeat try unfold_funcomp; auto_unfold in *; asimpl'; repeat try unfold_funcomp.
-
-Tactic Notation "asimpl" "in" hyp(J) := revert J; asimpl; intros J.
-
-Tactic Notation "auto_case" := auto_case (asimpl; cbn; eauto).
-
-Tactic Notation "asimpl" "in" "*" := auto_unfold in *; repeat first [progress rewrite ?instId_term in *| progress rewrite ?compComp_term in *| progress rewrite ?compComp'_term in *| progress rewrite ?instId_form in *| progress rewrite ?compComp_form in *| progress rewrite ?compComp'_form in *| progress rewrite ?varL_term in *| progress (unfold up_ren, up_term_term, upList_term_term in *)| progress (cbn [subst_term subst_form] in *)| fsimpl in *].
-
-Ltac substify := auto_unfold.
-
-Ltac renamify := auto_unfold.
+Notation "σ >> τ" := (seq_map (subst_term τ) σ) (at level 50, only parsing).
